CoFactor check to H2C

VRF/Hacl.VRF.HashToCurve.fst
@@ -15,6 +15,8 @@ open Spec.Lib.IntSeq.Lemmas
 open Spec.Lib.IntBuf.Lemmas
 open Hacl.VRF.Lib
 
+open Spec.Lib.RawIntTypes
+
 #set-options " --z3rlimit 200 "
 
 assume val hash: 
@@ -24,7 +26,6 @@ assume val hash:
 	Stack unit
 	(requires (fun h -> live h hashBuffer /\ live h input /\ disjoint hashBuffer input))
     (ensures (fun h0 _ h1 -> preserves_live h0 h1 /\ modifies1 hashBuffer h0 h1))
-
 
 assume val toU8: out: lbuffer uint8 16 -> input: uint128 -> 
 	Stack unit 
@@ -45,72 +46,108 @@ assume val decompress:
 		(requires (fun h -> live h out /\ live h input))
 		(ensures (fun h0 _ h1 -> preserves_live h0 h1 /\ modifies1 out h0 h1))
 
-noeq type uint256 = 
-	|C: high: uint_t U128 -> low: uint_t U128 -> uint256
+noeq type bignumCounter = 
+	|C: high: uint_t U128 -> low: uint_t U128 -> bignumCounter
 
-val v_counter: c: uint256 -> GTot nat 
-let v_counter c = 
-	let high = uint_v c.high in 
-	let low = uint_v c.low in 
-	pow2 128 * high + low
+val bignumCounterInc: b: bignumCounter{let h = uint_v b.high in let l = uint_v b.low in (pow2 128 * h + l) < pow2 256 -1} -> r: bignumCounter{
+	let h = uint_v r.high in let l = uint_v r.low in 
+	let h_ = uint_v b.high in let l_ = uint_v b.low in 
+	(pow2 128 * h_ + l_ ) + 1 = (pow2 128 * h + l)}
 
-assume val inc_: c: uint256{v_counter c < pow2 256 - 1} -> Tot (r: uint256{v_counter r = v_counter c + 1 })
+let bignumCounterInc b = 
+	let m = u128(0xffffffffffffffffffffffffffffffff) in 
+	let m_ = u128_to_UInt128 m in 
+	let one = u128_to_UInt128 (u128 1) in 
+	let zero = u128_to_UInt128 (u128 0) in 
+	let h = u128_to_UInt128 b.high in 
+	let l = u128_to_UInt128 b.low in 
+		if FStar.UInt128.eq l m_ then begin
+				assert_norm((pow2 128 -1) * pow2 128 = pow2 256 - pow2 128);
+			let h = FStar.UInt128.add h one in 
+			let l = zero in 
+			C (u128_from_UInt128 h) (u128_from_UInt128 l) 
+		end	
+		else
+			begin
+			let l = FStar.UInt128.add l one in 
+			C (u128_from_UInt128 h) (u128_from_UInt128 l) 
+			end
 
-assume val less: a: uint256 -> b: uint256 -> Tot bool
+(* TODO: *)
+
+assume val bignumCounterLess: b: bignumCounter -> c: bignumCounter -> Tot (r : bool {r == true ==> 
+	(let h = uint_v b.high in let l = uint_v b.low in 
+	let h_ = uint_v c.high in let l_ = uint_v c.low in 
+	(pow2 128 * h + l) < (pow2 128 * h_ + l_))})
+
+(* TODO: *)
+val pointCompare: a: point -> b: point -> Stack bool 
+	(requires (fun h0 -> live h0 a /\ live h0 b))
+	(ensures (fun h0 _ h1 -> preserves_live h0 h1))
+
+let pointCompare a b = 
+	let a0_i = (index a (size 0)) in 
+	let a0 = u128_to_UInt128 a0_i in 
+	let b0_i = (index b (size 0)) in 
+	let b0 = u128_to_UInt128 b0_i in  
+	let eq = FStar.UInt128.eq in 
+	eq a0 b0
 
 val _helper_ECVRF_hash_to_curve: 
 	#len : size_nat -> 
     pointBuffer : point -> 
-    output: lbuffer uint8 len-> (* length output = v inputLength + 96 *)
+    output: lbuffer uint8 len-> 
     clen:size_t{v clen = len /\ len >= 96} ->  
-    highCounter: uint128 -> 
-    lowCounter: uint128 -> 
+    counter: bignumCounter -> 
+    curveOrder: word -> 
+    curveOrderCounter: bignumCounter{bignumCounterLess counter curveOrderCounter == true /\ (
+    	let h = uint_v curveOrderCounter.high in let l = uint_v curveOrderCounter.low in 
+		(pow2 128 * h + l) < pow2 256 - 1)} -> 
+    cofactor_check_buffer: lbuffer uint128 40 -> 
     Stack bool
-        (requires (fun h0 -> live h0 pointBuffer /\live h0 output))
-   		(ensures (fun h0 _ h1 -> preserves_live h0 h1 /\ modifies2 output pointBuffer h0 h1 ))
+        (requires (fun h0 -> live h0 pointBuffer /\ live h0 output /\ live h0 cofactor_check_buffer /\ live h0 curveOrder /\ disjoint cofactor_check_buffer pointBuffer))
+		(ensures (fun h0 _ h1 -> preserves_live h0 h1)) 
 
-assume val greater: highCounter: uint128 -> lowCounter: uint128 -> highValue: uint128 -> lowValue: uint128 -> Tot bool
-
-(*let greater hc lc hv lv = 
-	if (highCounter > highValue) then true 
-	else if (highCounter < highValue) then false 
-	else
-		begin
-			if (lowCounter > lowValue) then true else false 
-		end	
-*)
-assume val inc: highCounter : uint128 -> lowCounter: uint128 -> Tot (tuple2 uint128 uint128)	 	
-
-let rec _helper_ECVRF_hash_to_curve #len pointBuffer output clen highCounter lowCounter  =
+let rec _helper_ECVRF_hash_to_curve #len pointBuffer output clen counter curveOrder curveOrderCounter cofactor_check_buffer = 
 	let inputLength = Spec.Lib.IntTypes.sub #SIZE clen (size 96) in 
-
 	let startBufferForCounter = add #SIZE inputLength (size 32) in 
-	let lengthBufferToInputHash = add #SIZE inputLength (size 64) in 
+	let lengthBufferToInputHash = add #SIZE inputLength (size 64) in
 
 	let bufferForInputHash = sub output (size 0) lengthBufferToInputHash in 
 	let bufferForComputedHash = sub output lengthBufferToInputHash (size 32) in 
-		
 	let placeForCounterHigh = sub output startBufferForCounter (size 16)   in
 	let placeForCounterLow = sub output (add #SIZE startBufferForCounter (size 16)) (size 16) in  
 
-	toU8 placeForCounterHigh highCounter;
-	toU8 placeForCounterLow lowCounter;
+	toU8 placeForCounterHigh counter.high;
+	toU8 placeForCounterLow counter.low;
 
-	hash bufferForComputedHash lengthBufferToInputHash bufferForInputHash;  
+	hash bufferForComputedHash lengthBufferToInputHash bufferForInputHash; 
 
   	let successful = decompress pointBuffer bufferForComputedHash in 
-  	if successful then true
-  	else
-  	( 
-  		(*Example *)
-  		let curveOrderHigh = u128 10 in 
-  		let curveOrderLow = u128 10 in 
-  		(*/Example *)
+  	if successful then 
+  		let buffer_point = sub cofactor_check_buffer (size 20) (size 20) in 
+  		disjoint_sub_lemma1 cofactor_check_buffer pointBuffer (size 20) (size 20);
+  		point_mult buffer_point pointBuffer curveOrder;
+  		let buffer_point_infinity = sub cofactor_check_buffer (size 0) (size 20) in 
+  		let r = pointCompare buffer_point buffer_point_infinity in 
+  		if r then 
+  			true
+  		else 
+  			begin
+  	  		let counterUpd = bignumCounterInc counter in 
+  			let rc = bignumCounterLess counterUpd curveOrderCounter in 
+  			if rc = false then false else 
+  				_helper_ECVRF_hash_to_curve #len pointBuffer output clen counterUpd curveOrder curveOrderCounter cofactor_check_buffer 
+  			end	
+  	else 
+  		begin
+  	  	let counterUpd = bignumCounterInc counter in 
+  		let rc = bignumCounterLess counterUpd curveOrderCounter in 
+  		if rc = false then false else 
+  			_helper_ECVRF_hash_to_curve #len pointBuffer output clen counterUpd curveOrder curveOrderCounter cofactor_check_buffer
+  	end
 
-  		if greater highCounter lowCounter curveOrderHigh curveOrderLow then false else
-  		let counterIncH, counterIncL = inc highCounter lowCounter in 
-  			_helper_ECVRF_hash_to_curve #len pointBuffer output clen highCounter lowCounter
-  )
+(*TODO: add the function checking whether curveOrder as word is the same as CurveOrderCounteryyy *)
 
 val _ECVRF_hash_to_curve:
 	#len:size_nat ->
@@ -118,26 +155,33 @@ val _ECVRF_hash_to_curve:
 	publicKey: point{disjoint pointBuffer publicKey}->
 	clen:size_t{v clen == len /\ len < maxint SIZE - 96} ->
 	input:lbuffer uint8 len ->
+	curveOrder: word -> 
+    curveOrderCounter: bignumCounter{let h = uint_v curveOrderCounter.high in let l = uint_v curveOrderCounter.low in (
+    	(pow2 128 * h + l) < pow2 256 - 1 && (pow2 128 * h + l > 0))} -> 
+    cofactor_check_buffer: lbuffer uint128 40 ->
 	Stack bool 
 		(requires
-			(fun h0 -> live h0 pointBuffer /\ live h0 input /\ live h0 publicKey)
+			(fun h0 -> live h0 pointBuffer /\ live h0 input /\ live h0 publicKey /\ live h0 cofactor_check_buffer /\ live h0 curveOrder /\ disjoint cofactor_check_buffer pointBuffer)
 		)
 		(ensures
-			(fun h0 _ h1 -> preserves_live h0 h1 /\ modifies1 pointBuffer h0 h1)
+			(fun h0 _ h1 -> preserves_live h0 h1)
 		)
 
-let _ECVRF_hash_to_curve #len pointBuffer publicKey clen input  = 
+let _ECVRF_hash_to_curve #len pointBuffer publicKey clen input curveOrder curveOrderCounter cofactor_check_buffer  = 
 	let sizeToHashBuffer = add #SIZE clen (size 96) in 
-	assert(uint_v sizeToHashBuffer >= 96);
 	let sizeInput = add #SIZE clen (size 32) in 
 	alloc #(uint8) #(bool) #(v sizeToHashBuffer) sizeToHashBuffer (u8(0)) 
-		[BufItem publicKey; BufItem input] [BufItem pointBuffer] 
+		[BufItem publicKey; BufItem input; BufItem curveOrder;] [BufItem pointBuffer; BufItem cofactor_check_buffer] 
 		(fun h0 _ h1 -> True) (
 			fun toHashBuffer ->  	
-					let inputBuffer = sub toHashBuffer (size 0) clen in 
+				let inputBuffer = sub toHashBuffer (size 0) clen in 
 				copy #_ #(v clen) clen input inputBuffer;
-
 	    		let compressedPublicKey = sub #_ #(v sizeToHashBuffer) #(32) toHashBuffer clen (size 32) in 
 				compress compressedPublicKey publicKey;
-				 _helper_ECVRF_hash_to_curve pointBuffer toHashBuffer sizeToHashBuffer (u128 0) (u128 0)
- 	)
+				let counterStart = C (u128 0) (u128 0) in 
+					assume (disjoint cofactor_check_buffer pointBuffer);	
+					assume (bignumCounterLess counterStart curveOrderCounter = true);
+				let r =  _helper_ECVRF_hash_to_curve pointBuffer toHashBuffer sizeToHashBuffer counterStart curveOrder curveOrderCounter cofactor_check_buffer in
+				admit(); 
+				r
+		)
